Update

SystemS.v
@@ -1,7 +1,9 @@
 Set Implicit Arguments.
 
+Definition rule (A : Set) := A -> option A.
+
 Inductive strategy (A : Set) : Set :=
-| SRule : (A -> option A) -> strategy A
+| SRule : rule A -> strategy A
 | SIdentity : strategy A
 | SFailure : strategy A
 | STest : strategy A -> strategy A
@@ -29,16 +31,16 @@ Inductive eval (A : Set) : strategy A -> A -> option A -> Prop :=
     forall s1 s2 t t' t'',
       eval s1 t (Some t') ->
       eval s2 t' (Some t'') ->
-      eval (s1;s2) t (Some t'')
+      eval (s1 ; s2) t (Some t'')
 | E_Seq2 :
     forall s1 s2 t,
       eval s1 t None ->
-      eval (s1;s2) t None
+      eval (s1 ; s2) t None
 | E_Seq3 :
     forall s1 s2 t t',
       eval s1 t (Some t') ->
       eval s2 t' None ->
-      eval (s1;s2) t None
+      eval (s1 ; s2) t None
 | E_LeftChoice1 :
     forall s1 s2 t t',
       eval s1 t (Some t') ->
@@ -66,12 +68,6 @@ Inductive eval (A : Set) : strategy A -> A -> option A -> Prop :=
       eval s1 t None ->
       eval s2 t None ->
       eval (SChoice s1 s2) t None.
-
-Definition succeeds A (s : strategy A) (t : A) : Prop :=
-  exists t', eval s t (Some t').
-
-Definition fails A (s : strategy A) (t : A) : Prop :=
-  eval s t None.
 
 Inductive without_choice A : strategy A -> Prop :=
 | WC_Rule : forall r, without_choice (SRule r)
@@ -121,4 +117,94 @@ Proof.
   try (apply IHs2 with t; assumption).
   assert (Some t' = None); apply IHs1 with t; congruence.
   assert (Some t'0 = None); apply IHs1 with t; congruence.
+Qed.
+
+
+Definition succeeds A (s : strategy A) (t : A) : Prop :=
+  exists t', eval s t (Some t').
+
+Definition fails A (s : strategy A) (t : A) : Prop :=
+  eval s t None.
+
+Definition orthogonal A (s1 s2 : strategy A) : Prop :=
+  forall t,
+    (forall t', eval s1 t (Some t') -> eval s2 t None) /\
+    (forall t', eval s2 t (Some t') -> eval s1 t None).
+
+Lemma orthogonal_cong1 :
+  forall A (s1 s2 : strategy A) t,
+    orthogonal s1 s2 -> succeeds s1 t -> fails s2 t.
+Proof.
+  firstorder.
+Qed.
+
+Lemma orthogonal_cong2 :
+  forall A (s1 s2 : strategy A) t,
+    orthogonal s1 s2 -> succeeds s2 t -> fails s1 t.
+Proof.
+  firstorder.
+Qed.
+
+Inductive is_orthogonal A : strategy A -> Prop :=
+| O_Rule : forall r, is_orthogonal (SRule r)
+| O_Id : is_orthogonal (SIdentity _)
+| O_Fail : is_orthogonal (SFailure _)
+| O_Test : forall s, is_orthogonal s -> is_orthogonal (STest s)
+| O_Neg : forall s, is_orthogonal s -> is_orthogonal (SNeg s)
+| O_Seq :
+    forall s1 s2,
+      is_orthogonal s1 ->
+      is_orthogonal s2 ->
+      is_orthogonal (s1 ; s2)
+| O_LeftChoice :
+    forall s1 s2,
+      is_orthogonal s1 ->
+      is_orthogonal s2 ->
+      is_orthogonal (s1 <+ s2)
+| O_Choice :
+    forall s1 s2,
+      orthogonal s1 s2 ->
+      is_orthogonal s1 ->
+      is_orthogonal s2 ->
+      is_orthogonal (SChoice s1 s2).
+
+Theorem is_orthogonal_deterministic :
+  forall A (s : strategy A),
+    is_orthogonal s -> deterministic s.
+Proof.
+  unfold deterministic;
+  induction s; intros Ho t x y Hx Hy;
+  inversion Ho; subst; clear Ho;
+
+  (* SRule, SIdentity, SFailure *)
+  try (inversion Hx; inversion Hy; subst; congruence);
+  
+  (* STest, SNeg *)
+  try (inversion Hx; inversion Hy; auto; subst;
+       assert (Some t' = None); apply IHs with t; congruence).
+
+  (* SSeq *)
+  inversion Hx; inversion Hy; auto; subst;
+  try (assert (Some t' = None); apply IHs1 with t; congruence);
+  try (assert (Some t'0 = Some t') as H by (apply IHs1 with t; assumption);
+       inversion H; subst; clear H;
+       apply IHs2 with t'; assumption).
+
+  (* SLeftChoice *)
+  inversion Hx; inversion Hy; auto; subst;
+  try (apply IHs1 with t; assumption);
+  try (apply IHs2 with t; assumption).
+  assert (Some t' = None); apply IHs1 with t; congruence.
+  assert (Some t'0 = None); apply IHs1 with t; congruence.
+
+  (* SChoice *)
+  inversion Hx; inversion Hy; auto; subst;
+  try (apply IHs1 with t; assumption);
+  try (apply IHs2 with t; assumption).
+  assert (eval s2 t None) by (apply orthogonal_cong1 with s1; firstorder);
+    assert (Some t'0 = None) by (apply IHs2 with t; assumption);
+    congruence.
+  assert (eval s1 t None) by (apply orthogonal_cong2 with s2; firstorder);
+    assert (Some t'0 = None) by (apply IHs1 with t; assumption);
+    congruence.
 Qed.
